proofs/arch/arch_extra.v
@@ -248,8 +248,8 @@ End ARCH.
 (* Extra ops are non-existing architecture-specific asm instructions that we
  * replace by real asm instructions during the asmgen pass.
  *)
-Class asm_extra (reg regx xreg rflag cond asm_op extra_op : Type) :=
-  { _asm   : asm reg regx xreg rflag cond asm_op
+Class asm_extra (reg regx xreg regmask rflag cond asm_op extra_op : Type) :=
+  { _asm   : asm reg regx xreg regmask rflag cond asm_op
   ; _atoI  : arch_toIdent
   ; _extra : asmOp extra_op (* description of extra ops *)
   (* How to compile extra ops into a assembly instructions. *)
@@ -264,7 +264,7 @@ Class asm_extra (reg regx xreg rflag cond asm_op extra_op : Type) :=
 #[global]
 Existing Instances _asm _atoI _extra.
 
-Definition extra_op_t {reg regx xreg rflag cond asm_op extra_op} {asm_e : asm_extra reg regx xreg rflag cond asm_op extra_op} := extra_op.
+Definition extra_op_t {reg regx xreg regmask rflag cond asm_op extra_op} {asm_e : asm_extra reg regx xreg regmask rflag cond asm_op extra_op} := extra_op.
 
 Section AsmOpI.
 
